ulib/FStar.Reflection.Types.fsti
@@ -4,3 +4,4 @@ assume new type binder
 assume new type term
 assume new type env
 assume new type fv
+assume new type bv
